lib/Buckets/KVList.i.dfy
@@ -1,10 +1,9 @@
-include "../lib/Base/Message.i.dfy"
-include "../lib/Base/sequences.i.dfy"
-include "../lib/Base/Maps.s.dfy"
-include "../lib/Base/NativeArrays.s.dfy"
-include "../PivotBetree/BucketsLib.i.dfy"
-include "../PivotBetree/BucketWeights.i.dfy"
-include "../lib/Marshalling/Seqs.i.dfy"
+include "../Base/Message.i.dfy"
+include "../Base/sequences.i.dfy"
+include "../Base/Maps.s.dfy"
+include "../Base/NativeArrays.s.dfy"
+include "BucketsLib.i.dfy"
+include "BucketWeights.i.dfy"
 //
 // A list of key-message pairs, with unique, sorted keys.
 // TODO(robj,thance): How is it used... in BucketImpl?
